theories/rules/rules_EInit.v
@@ -41,7 +41,7 @@ Section cap_lang_rules.
       EInit_fail lregs lmem ot.
 
   Inductive EInit_spec (lregs lregs' : LReg) (lmem lmem' : LMem) (n n' : nat) (tidx : TIndex) (eid : EIdentity) (ot : OType) (rs : RegName) : cap_lang.val → Prop :=
-    | EInit_success_no_revoke code_b code_e code_a code_v data_b data_e data_a data_v vmap :
+    | EInit_success_no_revoke code_b code_e code_a code_v data_b data_e data_a data_v :
       incrementLPC lregs = Some lregs' → (* PC can be incremented *)
       n + 1 = n' → (* n is the value of the EC register, it can be incremented to n' *)
       tidx = n →
@@ -51,8 +51,9 @@ Section cap_lang_rules.
       lmem !! (code_b, code_v) = Some (LCap RW data_b data_e data_a data_v) → (* the base address of the code capability points to a valid data capability *)
       is_valid_updated_lmemory lmem (finz.seq_between code_b code_e) code_v lmem' → (* support revocation *) (* all memory in the code capability is "current" w.r.t. revocation *)
       is_valid_updated_lmemory lmem (finz.seq_between data_b data_e) data_v lmem' → (* support revocation *) (* all memory in the data capability is "current" w.r.t. revocation *)
-      unique_in_registersL lregs rs (LCap RX code_b code_e code_a code_v) → (* the code capability in the rs register is unique across all other registers *)
-      unique_in_memoryL lmem vmap (LCap RW data_b data_e data_a data_v) → (* the data capability at base address b of the code capability is unique across all of memory *)
+      unique_in_registersL lregs (Some rs) (LCap RX code_b code_e code_a code_v) → (* the code capability in the rs register is unique across all other registers *)
+      unique_in_registersL lregs None (* no excluded register this time *) (LCap RW data_b data_e data_a data_v) → (* the data capability in the rs register is unique across all other registers *)
+      (* TODO: missing above: need to exclude the capability at b itself, cannot just sweep all of memory *)
       incrementLPC (<[ rs := next_version_lword (LCap E code_b code_e (code_b ^+ 1)%a code_v)]> lregs) = Some lregs' → (* the pc will be incremented and rs will point to a "current" sentry capability *)
       EInit_spec lregs lregs' lmem lmem' n n' tidx eid ot rs NextIV
     | EInit_failure :
